Weidenbach_Book/IsaSAT/IsaSAT_Setup2_LLVM.thy
@@ -1,5 +1,6 @@
 theory IsaSAT_Setup2_LLVM
   imports IsaSAT_Setup
+    IsaSAT_Bump_Heuristics_LLVM
     IsaSAT_Setup0_LLVM
 begin
 
@@ -484,12 +485,6 @@ lemmas [sepref_fr_rules] = watched_by_app.refine watched_by_app.XX.mop_refine
 lemmas [unfolded inline_direct_return_node_case, llvm_code] =
   length_ll_fs_heur_fast_code_def[unfolded read_all_st_code_def]
 
-sepref_def isa_vmtf_heur_fst_code
-  is \<open>isa_vmtf_heur_fst\<close>
-  :: \<open>heuristic_bump_assn\<^sup>k \<rightarrow>\<^sub>a atom_assn\<close>
-  unfolding isa_vmtf_heur_fst_def
-  by sepref
-
 definition get_vmtf_heur_fst_impl where
   \<open>get_vmtf_heur_fst_impl = read_vmtf_wl_heur_code (isa_vmtf_heur_fst_code)\<close>
 
@@ -511,24 +506,24 @@ global_interpretation vmtf_fst: read_vmtf_param_adder0 where
   done
 
 definition get_bump_heur_array_nth_impl where
-  \<open>get_bump_heur_array_nth_impl N C' = read_vmtf_wl_heur_code (\<lambda>M. vmtf_heur_array_nth_code M C') N\<close>
+  \<open>get_bump_heur_array_nth_impl N C' = read_vmtf_wl_heur_code (\<lambda>M. isa_vmtf_heur_array_nth_code M C') N\<close>
 
 global_interpretation vmtf_array_nth: read_vmtf_param_adder where
-  f' = \<open>\<lambda>a b. vmtf_heur_array_nth b a\<close> and
-  f = \<open>\<lambda>a b. vmtf_heur_array_nth_code b a\<close> and
+  f' = \<open>\<lambda>a b. isa_vmtf_heur_array_nth b a\<close> and
+  f = \<open>\<lambda>a b. isa_vmtf_heur_array_nth_code b a\<close> and
   x_assn = vmtf_node_assn and
-  P = \<open>(\<lambda>n S. n < length (fst (fst S)))\<close> and
+  P = \<open>(\<lambda>n S. n < length (fst (bump_get_heuristics S)))\<close> and
   R = atom_rel
  rewrites
-    \<open>(\<lambda>N C'. read_vmtf_wl_heur (\<lambda>M. vmtf_heur_array_nth M C') N) = RETURN oo get_bump_heur_array_nth\<close>  and
-    \<open>(\<lambda>N C'. read_vmtf_wl_heur_code (\<lambda>M. vmtf_heur_array_nth_code M C') N) = get_bump_heur_array_nth_impl\<close>
+    \<open>(\<lambda>N C'. read_vmtf_wl_heur (\<lambda>M. isa_vmtf_heur_array_nth M C') N) = RETURN oo get_bump_heur_array_nth\<close>  and
+    \<open>(\<lambda>N C'. read_vmtf_wl_heur_code (\<lambda>M. isa_vmtf_heur_array_nth_code M C') N) = get_bump_heur_array_nth_impl\<close>
   apply unfold_locales
   apply (subst (3)uncurry_def)
-  apply (rule vmtf_heur_array_nth_code.refine)
+  apply (rule isa_vmtf_heur_array_nth_code.refine)
   subgoal
     by (auto intro!: ext simp: get_bump_heur_array_nth_def read_all_st_def vmtf_heur_array_nth_def
-        get_vmtf_heur_array_def
-       split: isasat_int_splits)
+        get_vmtf_heur_array_def isa_vmtf_heur_array_nth_def bump_get_heuristics_def
+      split: isasat_int_splits bump_heuristics_splits prod.splits)
   subgoal by (auto simp: get_bump_heur_array_nth_impl_def[abs_def])
   done
 
@@ -567,7 +562,7 @@ sepref_def mop_mark_added_heur_st_impl
 
 experiment
 begin
-term empty_search_stats_impl
+
 export_llvm opts_reduction_st_fast_code opts_restart_st_fast_code opts_unbounded_mode_st_fast_code
   opts_minimum_between_restart_st_fast_code mop_arena_status_st_impl full_arena_length_st_impl
   get_global_conflict_count_impl get_count_max_lvls_heur_impl clss_size_resetUS0_st
